Adjusted files to handle stratified prophecies

theories/typing/mod_ty.v
@@ -4,8 +4,16 @@ Set Default Proof Using "Type".
 
 Implicit Type 𝔄 𝔅 ℭ: syn_type.
 
+Global Instance compose_inj {A B C} f `{Inj A B (=) (=) f} : @Inj (C → A) (C → B) (=) (=) (compose f).
+Proof. intros ???. fun_ext. intros ?. apply (inj f). specialize (equal_f H0 x0). done. Qed.
+
 Section mod_ty.
   Context `{!typeG Σ}.
+
+  Class SameLevel 𝔄 𝔅 : Prop := {same_level: ghost_level 𝔅 = ghost_level 𝔄}.
+
+  Global Instance same_level_refl 𝔄 : SameLevel 𝔄 𝔄.
+  Proof. done. Qed. 
 
   Lemma split_mt_mod_ty {𝔄 𝔅} (f: 𝔄 → 𝔅) ty vπ' d tid l :
     (l ↦∗: λ vl, ∃vπ, ⌜vπ' = f ∘ vπ⌝ ∗ ty.(ty_own) vπ d tid vl) ⊣⊢
@@ -17,8 +25,9 @@ Section mod_ty.
       by iSplit; [done|].
   Qed.
 
-  Program Definition mod_ty {𝔄 𝔅} (f: 𝔄 → 𝔅) (ty: type 𝔄) : type 𝔅 := {|
-    ty_size := ty.(ty_size);  ty_lfts := ty.(ty_lfts);  ty_E := ty.(ty_E);
+  Program Definition mod_ty `{SameLevel 𝔄 𝔅} (f: 𝔄 → 𝔅) (ty: type 𝔄) : type 𝔅 := {|
+    ty_size := ty.(ty_size);  ty_lfts := ty.(ty_lfts);  ty_E := ty.(ty_E); 
+    ty_proph vπ ξl := exists vπ', vπ = f ∘ vπ' /\ ty.(ty_proph) vπ' ξl;
     ty_own vπ d tid vl := ∃vπ', ⌜vπ = f ∘ vπ'⌝ ∗ ty.(ty_own) vπ' d tid vl;
     ty_shr vπ d κ tid l := ∃vπ', ⌜vπ = f ∘ vπ'⌝ ∗ ty.(ty_shr) vπ' d κ tid l;
   |}%I.
@@ -46,7 +55,7 @@ Section mod_ty.
     move=> */=. iIntros "#LFT In [%vπ[->ty]] κ".
     iMod (ty_own_proph with "LFT In ty κ") as "Upd"; [done|]. iModIntro.
     iApply (step_fupdN_wand with "Upd"). iMod 1 as (ξl q ?) "[ξl Toty]".
-    iModIntro. iExists ξl, q. iSplit; [iPureIntro; by apply (proph_dep_constr _)|].
+    iModIntro. iExists ξl, q. iSplit; [by iExists _|].
     iIntros "{$ξl}ξl". iMod ("Toty" with "ξl") as "[? $]".
     iModIntro. iExists vπ. by iSplit.
   Qed.
@@ -54,11 +63,12 @@ Section mod_ty.
     move=> */=. iIntros "#LFT In In' [%vπ[->ty]] κ".
     iMod (ty_shr_proph with "LFT In In' ty κ") as "Upd"; [done|]. iIntros "!>!>".
     iApply (step_fupdN_wand with "Upd"). iMod 1 as (ξl q ?) "[ξl Toκ]".
-    iModIntro. iExists ξl, q. iSplit; [iPureIntro; by apply (proph_dep_constr _)|].
+    iModIntro. iExists ξl, q. iSplit; [by iExists _|].
     iIntros "{$ξl}ξl". by iMod ("Toκ" with "ξl").
   Qed.
+  Next Obligation. move=> /= ???????[?[->?]]. rewrite same_level. by eapply proph_dep_constr, ty_proph_weaken. Qed.
 
-  Global Instance mod_ty_ne {𝔄 𝔅} (f: 𝔄 → 𝔅) : NonExpansive (mod_ty f).
+  Global Instance mod_ty_ne `{SameLevel 𝔄 𝔅} (f: 𝔄 → 𝔅) : NonExpansive (mod_ty f).
   Proof. solve_ne_type. Qed.
 End mod_ty.
 
@@ -67,45 +77,55 @@ Notation "<{ f }>" := (mod_ty f) (format "<{ f }>"): lrust_type_scope.
 Section typing.
   Context `{!typeG Σ}.
 
-  Lemma mod_ty_own' {𝔄 𝔅} g f `{!@SemiIso 𝔄 𝔅 f g} ty vπ d tid vl :
+  Lemma mod_ty_own' `{SameLevel 𝔄 𝔅} g f `{!@SemiIso 𝔄 𝔅 f g} ty vπ d tid vl :
     (<{f}> ty).(ty_own) vπ d tid vl ⊢ ty.(ty_own) (g ∘ vπ) d tid vl.
   Proof. iIntros "[%[->?]]". by rewrite compose_assoc semi_iso. Qed.
-  Lemma mod_ty_own {𝔄 𝔅} g f `{!@Iso 𝔄 𝔅 f g} ty vπ d tid vl :
+  Lemma mod_ty_own `{SameLevel 𝔄 𝔅} g f `{!@Iso 𝔄 𝔅 f g} ty vπ d tid vl :
     (<{f}> ty).(ty_own) vπ d tid vl ⊣⊢ ty.(ty_own) (g ∘ vπ) d tid vl.
   Proof.
     iSplit; [by iApply mod_ty_own'|]. iIntros "ty". iExists _. iFrame "ty".
     by rewrite compose_assoc semi_iso.
   Qed.
 
-  Lemma mod_ty_shr' {𝔄 𝔅} g f `{!@SemiIso 𝔄 𝔅 f g} ty vπ d κ tid l :
+  Lemma mod_ty_shr' `{SameLevel 𝔄 𝔅} g f `{!@SemiIso 𝔄 𝔅 f g} ty vπ d κ tid l :
     (<{f}> ty).(ty_shr) vπ d κ tid l ⊢ ty.(ty_shr) (g ∘ vπ) d κ tid l.
   Proof. iIntros "[%[->?]]". by rewrite compose_assoc semi_iso. Qed.
-  Lemma mod_ty_shr {𝔄 𝔅} g f `{!@Iso 𝔄 𝔅 f g} ty vπ d κ tid l :
+  Lemma mod_ty_shr `{SameLevel 𝔄 𝔅} g f `{!@Iso 𝔄 𝔅 f g} ty vπ d κ tid l :
     (<{f}> ty).(ty_shr) vπ d κ tid l ⊣⊢ ty.(ty_shr) (g ∘ vπ) d κ tid l.
   Proof.
     iSplit; [by iApply mod_ty_shr'|]. iIntros "ty". iExists _. iFrame "ty".
     by rewrite compose_assoc semi_iso.
   Qed.
 
-  Global Instance mod_ty_type_ne {𝔄 𝔅} (f: 𝔄 → 𝔅) : TypeNonExpansive <{f}>%T.
+  Lemma mod_ty_proph' `{SameLevel 𝔄 𝔅} g f `{!@SemiIso 𝔄 𝔅 f g} ty vπ ξl :
+    (<{f}> ty).(ty_proph) vπ ξl → ty.(ty_proph) (g ∘ vπ) ξl.
+  Proof. intros [? [-> ?]]. by rewrite compose_assoc semi_iso. Qed.
+  Lemma mod_ty_proph `{SameLevel 𝔄 𝔅} g f `{!@Iso 𝔄 𝔅 f g} ty vπ ξl :
+    (<{f}> ty).(ty_proph) vπ ξl ↔ ty.(ty_proph) (g ∘ vπ) ξl.
   Proof.
-    split=>/= *; by [apply type_lft_morphism_id_like| |do 3 f_equiv|do 3 f_equiv].
+    split; [apply mod_ty_proph'; apply H0|]. intros ty_p. eexists _. split; [|done].
+    by rewrite compose_assoc semi_iso.
   Qed.
 
-  Global Instance mod_ty_copy {𝔄 𝔅} (f: 𝔄 → 𝔅) ty : Copy ty → Copy (<{f}> ty).
+  Global Instance mod_ty_type_ne `{SameLevel 𝔄 𝔅} (f: 𝔄 → 𝔅) : TypeNonExpansive <{f}>%T.
+  Proof.
+    split; simpl; intros; [apply type_lft_morphism_id_like| |do 3 f_equiv|do 3 f_equiv|do 3 f_equiv]; try done. apply H0.
+  Qed.
+
+  Global Instance mod_ty_copy `{SameLevel 𝔄 𝔅} (f: 𝔄 → 𝔅) ty : Copy ty → Copy (<{f}> ty).
   Proof.
     move=> [? ShrAcc]. split; [by apply _|]=> */=. iIntros "LFT [%vπ[->ty]] Na κ".
     iMod (ShrAcc with "LFT ty Na κ") as (q vl) "($& ↦ &?& Toκ)"; [done|done|].
     iModIntro. iExists q, vl. iFrame "↦ Toκ". iNext. iExists vπ. by iSplit.
   Qed.
 
-  Global Instance mod_ty_send {𝔄 𝔅} (f: 𝔄 → 𝔅) ty : Send ty → Send (<{f}> ty).
+  Global Instance mod_ty_send `{SameLevel 𝔄 𝔅} (f: 𝔄 → 𝔅) ty : Send ty → Send (<{f}> ty).
   Proof. move=> ?>/=. by do 3 f_equiv. Qed.
 
-  Global Instance mod_ty_sync {𝔄 𝔅} (f: 𝔄 → 𝔅) ty : Sync ty → Sync (<{f}> ty).
+  Global Instance mod_ty_sync `{SameLevel 𝔄 𝔅} (f: 𝔄 → 𝔅) ty : Sync ty → Sync (<{f}> ty).
   Proof. move=> ?>/=. by do 3 f_equiv. Qed.
 
-  Lemma mod_ty_resolve' {𝔄 𝔅} E L (f: 𝔄 → 𝔅) ty Φ :
+  Lemma mod_ty_resolve' `{SameLevel 𝔄 𝔅} E L (f: 𝔄 → 𝔅) ty Φ :
     resolve E L ty Φ → resolve E L (<{f}> ty) (λ b, ∃a, b = f a ∧ Φ a).
   Proof.
     move=> Rslv > ?. iIntros "LFT PROPH E L (%&->& ty)".
@@ -114,18 +134,18 @@ Section typing.
     iApply proph_obs_impl; [|done]=>/= ??. by eexists _.
   Qed.
 
-  Lemma mod_ty_resolve {𝔄 𝔅} E L f g `{!@SemiIso 𝔄 𝔅 f g} ty Φ :
+  Lemma mod_ty_resolve `{SameLevel 𝔄 𝔅} E L f g `{!@SemiIso 𝔄 𝔅 f g} ty Φ :
     resolve E L ty Φ → resolve E L (<{f}> ty) (Φ ∘ g).
   Proof.
     move=> ?. eapply resolve_impl; [by apply mod_ty_resolve'|]=>/=
     ?[?[/(f_equal g) + ?]]. by rewrite semi_iso'=> ->.
   Qed.
 
-  Lemma mod_ty_resolve_just {𝔄 𝔅} E L (f: 𝔄 → 𝔅) ty :
+  Lemma mod_ty_resolve_just `{SameLevel 𝔄 𝔅} E L (f: 𝔄 → 𝔅) ty :
     resolve E L ty (const True) → resolve E L (<{f}> ty) (const True).
   Proof. move=> ?. apply resolve_just. Qed.
 
-  Lemma mod_ty_real {𝔄 𝔅 ℭ} E L f g `{!@Iso 𝔄 𝔅 f g} (h: _ → ℭ) ty :
+  Lemma mod_ty_real `{SameLevel 𝔄 𝔅} {ℭ} E L f g `{!@Iso 𝔄 𝔅 f g} (h: _ → ℭ) ty :
     real E L ty h → real E L (<{f}> ty) (h ∘ g).
   Proof.
     move=> [Rlo Rls]. split.
@@ -138,50 +158,60 @@ Section typing.
   Qed.
 
   Lemma mod_ty_id {𝔄} (ty: type 𝔄) : <{id}>%T ty ≡ ty.
-  Proof. split; move=>// *; by [rewrite mod_ty_own|rewrite mod_ty_shr]. Qed.
+  Proof. split; move=>// *; by [rewrite mod_ty_proph|rewrite mod_ty_own|rewrite mod_ty_shr]. Qed.
 
-  Lemma mod_ty_compose {𝔄 𝔅 ℭ} (f: 𝔄 → 𝔅) (g: 𝔅 → ℭ) ty :
+  Local Instance same_level_trans 𝔄 𝔅 ℭ `{SameLevel 𝔄 𝔅} `{SameLevel 𝔅 ℭ} : SameLevel 𝔄 ℭ.
+  Proof. eassert (_ = _); [|done]. transitivity (ghost_level 𝔅); apply same_level. Qed. 
+
+  Lemma mod_ty_compose `{SameLevel 𝔄 𝔅} `{SameLevel 𝔅 ℭ} (f: 𝔄 → 𝔅) (g: 𝔅 → ℭ) ty :
     (<{g}> (<{f}> ty) ≡ <{g ∘ f}> ty)%T.
   Proof.
-    split=>// *; (iSplit=>/=; [
+    split=>// *; [shelve | |]; (iSplit=>/=; [
       iIntros "(%&->& %vπ &->&?)"; iExists vπ; by iFrame|
       iIntros "[%vπ[->?]]"; iExists (f ∘ vπ); (iSplit; [done|]); iExists vπ; by iFrame
     ]).
+    Unshelve. split.
+    intros (?&->&?&->&?). eexists; split; [|done]. by rewrite compose_assoc.
+    intros (?&->&?). eexists; split. done. eexists; split; [|done]. done.
   Qed.
 
-  Lemma mod_ty_in {𝔄 𝔅} E L (f: 𝔄 → 𝔅) ty : subtype E L ty (<{f}> ty) f.
+  Lemma mod_ty_in `{SameLevel 𝔄 𝔅} E L (f: 𝔄 → 𝔅) `{Inj _ _ (=) (=) f} ty : subtype E L ty (<{f}> ty) f.
   Proof.
-    iIntros "*_!>_". iSplit; [done|]. iSplit; [by iApply lft_incl_refl|].
+    iIntros "*_!>_". iSplit. iPureIntro. split. done.
+    intros ?? (?&?&?). apply compose_inj in H1; [|done]. by rewrite H1.
+    iSplit; [by iApply lft_incl_refl|].
     iSplit; iIntros "!>" (vπ) "*?"; iExists vπ; by iSplit.
   Qed.
 
-  Lemma mod_ty_out {𝔄 𝔅} E L f g `{!@SemiIso 𝔄 𝔅 f g} ty :
+  Lemma mod_ty_out `{SameLevel 𝔄 𝔅} E L f g `{!@Iso 𝔄 𝔅 f g} ty :
     subtype E L (<{f}> ty) ty g.
   Proof.
-    iIntros "*_!>_". iSplit; [done|]. iSplit; [by iApply lft_incl_refl|].
+    iIntros "*_!>_".
+    iSplit. iPureIntro. split; [done|]. intros. exists (g ∘ vπ). by rewrite compose_assoc semi_iso.
+    iSplit; [by iApply lft_incl_refl|].
     iSplit; iIntros "!>*/=[%[->?]]"; by rewrite compose_assoc semi_iso.
   Qed.
 
-  Lemma mod_ty_inout {𝔄 𝔅} E L f g `{!@SemiIso 𝔄 𝔅 f g} ty :
+  Lemma mod_ty_inout `{SameLevel 𝔄 𝔅} E L f g `{!@Iso 𝔄 𝔅 f g} ty :
     eqtype E L ty (<{f}> ty) f g.
-  Proof. by split; [apply mod_ty_in|apply mod_ty_out]. Qed.
-  Lemma mod_ty_outin {𝔄 𝔅} E L f g `{!@SemiIso 𝔄 𝔅 f g} ty :
+  Proof. split; by [apply mod_ty_in; apply semi_iso_inj |apply mod_ty_out]. Qed.
+  Lemma mod_ty_outin `{SameLevel 𝔄 𝔅} E L f g `{!@Iso 𝔄 𝔅 f g} ty :
     eqtype E L (<{f}> ty) ty g f.
   Proof. by apply eqtype_symm, mod_ty_inout. Qed.
 
-  Lemma mod_ty_subtype {𝔄 𝔅 𝔄' 𝔅'} E L h
-      f (f': 𝔄' → 𝔅') g `{!@SemiIso 𝔄 𝔅 f g} ty ty' :
+  Lemma mod_ty_subtype `{SameLevel 𝔄 𝔅} `{SameLevel 𝔄' 𝔅'} E L h
+      f f' `{Inj 𝔄' 𝔅' (=) (=) f'} g `{!@Iso 𝔄 𝔅 f g} ty ty' :
     subtype E L ty ty' h → subtype E L (<{f}> ty) (<{f'}> ty') (f' ∘ h ∘ g).
   Proof.
     move=> ??. eapply subtype_trans; [by apply mod_ty_out|].
     eapply subtype_trans; by [|apply mod_ty_in].
   Qed.
 
-  Lemma mod_ty_eqtype {𝔄 𝔅 𝔄' 𝔅'} E L h h' f f' g g'
-      `{!@SemiIso 𝔄 𝔅 f g} `{!@SemiIso 𝔄' 𝔅' f' g'} ty ty' :
+  Lemma mod_ty_eqtype `{SameLevel 𝔄 𝔅} `{SameLevel 𝔄' 𝔅'} E L h h' f f' g g'
+      `{!@Iso 𝔄 𝔅 f g} `{!@Iso 𝔄' 𝔅' f' g'} ty ty' :
     eqtype E L ty ty' h h' →
     eqtype E L (<{f}> ty) (<{f'}> ty') (f' ∘ h ∘ g) (f ∘ h' ∘ g').
-  Proof. move=> [??]. split; by apply mod_ty_subtype. Qed.
+  Proof. move=> [??]. split; apply mod_ty_subtype; try done; apply semi_iso_inj. Qed.
 End typing.
 
 Global Hint Resolve mod_ty_in mod_ty_out mod_ty_inout mod_ty_outin
