theories/typing/base_type.v
@@ -11,25 +11,29 @@ Section base.
   Context `{!typeG Σ}.
 
   Program Definition base {𝔄} : type 𝔄 :=
-    {| pt_size := 0; pt_own _ _ _ := False |}%I.
+    {| st_size := 0; st_lfts := [];  st_E := [];
+       st_proph _ _ := false; st_own _ _ _ _ := False |}%I.
   Next Obligation. by iIntros. Qed.
+  Next Obligation. done. Qed.
+  Next Obligation. by iIntros. Qed.
+  Next Obligation. done. Qed.
 
   Global Instance base_send {𝔄} : Send (@base 𝔄).
   Proof. done. Qed.
 
   Lemma base_resolve {𝔄} E L Φ : resolve E L (@base 𝔄) Φ.
-  Proof. by iIntros "* _ _ _ _" ([?[??]]). Qed.
+  Proof. iIntros "* _ _ _ _" ([]). Qed.
 
   Lemma base_real {𝔄 𝔅} E L (f: 𝔄 → 𝔅) : real E L base f.
   Proof.
     split.
-    - iIntros "*% _ _ _ (%&_&[])".
-    - iIntros "*% _ _ _ (%&_& own) !>!>". iDestruct "own" as (?) "[_[]]".
+    - iIntros "*% _ _ _" ([]).
+    - by iIntros "*% _ _ _ (%x&_&>%)".
   Qed.
 
   Lemma base_subtype {𝔄 𝔅} (f: 𝔄 → 𝔅) E L : subtype E L base base f.
   Proof.
-    apply subtype_plain_type. iIntros "*_!>_/=". iSplit; [done|].
+    apply subtype_simple_type. simpl. iIntros "*_!>_/=". iSplit; [done|].
     iSplit; [iApply lft_incl_refl|by iIntros].
   Qed.
   Lemma base_eqtype {𝔄 𝔅} (f: 𝔄 → 𝔅) g E L : eqtype E L base base f g.
