theories/typing/int.v
@@ -18,7 +18,8 @@ Section int.
 
   Lemma bool_ty_to_int E L : subtype E L bool_ty int Z_of_bool.
   Proof.
-    apply subtype_plain_type. iIntros "*_!>_/=". iSplit; [done|].
+    apply subtype_plain_type. intros ???; destruct x; destruct y; simpl in H; done.
+    iIntros "*_!>_/=". iSplit; [done|].
     iSplit; [iApply lft_incl_refl|]. by iIntros.
   Qed.
 
